examples/verifythis_fm2012_treedel/verifythis_fm2012_treedel_Treedel_main_lemma_1.v
@@ -2,11 +2,35 @@
 (* Beware! Only edit allowed sections below    *)
 Require Import BuiltIn.
 Require BuiltIn.
-Require map.Map.
 Require int.Int.
 
 (* Why3 assumption *)
-Definition unit := unit.
+Definition unit  := unit.
+
+Axiom map : forall (a:Type) {a_WT:WhyType a} (b:Type) {b_WT:WhyType b}, Type.
+Parameter map_WhyType : forall (a:Type) {a_WT:WhyType a}
+  (b:Type) {b_WT:WhyType b}, WhyType (map a b).
+Existing Instance map_WhyType.
+
+Parameter get: forall {a:Type} {a_WT:WhyType a} {b:Type} {b_WT:WhyType b},
+  (map a b) -> a -> b.
+
+Parameter set: forall {a:Type} {a_WT:WhyType a} {b:Type} {b_WT:WhyType b},
+  (map a b) -> a -> b -> (map a b).
+
+Axiom Select_eq : forall {a:Type} {a_WT:WhyType a} {b:Type} {b_WT:WhyType b},
+  forall (m:(map a b)), forall (a1:a) (a2:a), forall (b1:b), (a1 = a2) ->
+  ((get (set m a1 b1) a2) = b1).
+
+Axiom Select_neq : forall {a:Type} {a_WT:WhyType a}
+  {b:Type} {b_WT:WhyType b}, forall (m:(map a b)), forall (a1:a) (a2:a),
+  forall (b1:b), (~ (a1 = a2)) -> ((get (set m a1 b1) a2) = (get m a2)).
+
+Parameter const: forall {a:Type} {a_WT:WhyType a} {b:Type} {b_WT:WhyType b},
+  b -> (map a b).
+
+Axiom Const : forall {a:Type} {a_WT:WhyType a} {b:Type} {b_WT:WhyType b},
+  forall (b1:b) (a1:a), ((get (const b1:(map a b)) a1) = b1).
 
 (* Why3 assumption *)
 Inductive ref (a:Type) {a_WT:WhyType a} :=
@@ -16,46 +40,43 @@ Existing Instance ref_WhyType.
 Implicit Arguments mk_ref [[a] [a_WT]].
 
 (* Why3 assumption *)
-Definition contents {a:Type} {a_WT:WhyType a} (v:(ref a)): a :=
+Definition contents {a:Type} {a_WT:WhyType a}(v:(ref a)): a :=
   match v with
   | (mk_ref x) => x
   end.
 
-Axiom pointer : Type.
-Parameter pointer_WhyType : WhyType pointer.
-Existing Instance pointer_WhyType.
+Axiom loc : Type.
+Parameter loc_WhyType : WhyType loc.
+Existing Instance loc_WhyType.
 
-Parameter null: pointer.
+Parameter null: loc.
 
 (* Why3 assumption *)
-Inductive node :=
-  | mk_node : pointer -> pointer -> Z -> node.
+Inductive node  :=
+  | mk_node : loc -> loc -> Z -> node .
 Axiom node_WhyType : WhyType node.
 Existing Instance node_WhyType.
 
 (* Why3 assumption *)
-Definition data (v:node): Z := match v with
+Definition data(v:node): Z := match v with
   | (mk_node x x1 x2) => x2
   end.
 
 (* Why3 assumption *)
-Definition right1 (v:node): pointer :=
-  match v with
+Definition right1(v:node): loc := match v with
   | (mk_node x x1 x2) => x1
   end.
 
 (* Why3 assumption *)
-Definition left1 (v:node): pointer :=
-  match v with
+Definition left1(v:node): loc := match v with
   | (mk_node x x1 x2) => x
   end.
 
 (* Why3 assumption *)
-Definition memory := (map.Map.map pointer node).
+Definition memory  := (map loc node).
 
 (* Why3 assumption *)
-Inductive tree
-  (a:Type) {a_WT:WhyType a} :=
+Inductive tree (a:Type) {a_WT:WhyType a} :=
   | Empty : tree a
   | Node : (tree a) -> a -> (tree a) -> tree a.
 Axiom tree_WhyType : forall (a:Type) {a_WT:WhyType a}, WhyType (tree a).
@@ -64,8 +85,7 @@ Implicit Arguments Empty [[a] [a_WT]].
 Implicit Arguments Node [[a] [a_WT]].
 
 (* Why3 assumption *)
-Inductive list
-  (a:Type) {a_WT:WhyType a} :=
+Inductive list (a:Type) {a_WT:WhyType a} :=
   | Nil : list a
   | Cons : a -> (list a) -> list a.
 Axiom list_WhyType : forall (a:Type) {a_WT:WhyType a}, WhyType (list a).
@@ -74,7 +94,7 @@ Implicit Arguments Nil [[a] [a_WT]].
 Implicit Arguments Cons [[a] [a_WT]].
 
 (* Why3 assumption *)
-Fixpoint infix_plpl {a:Type} {a_WT:WhyType a} (l1:(list a)) (l2:(list
+Fixpoint infix_plpl {a:Type} {a_WT:WhyType a}(l1:(list a)) (l2:(list
   a)) {struct l1}: (list a) :=
   match l1 with
   | Nil => l2
@@ -89,7 +109,7 @@ Axiom Append_l_nil : forall {a:Type} {a_WT:WhyType a}, forall (l:(list a)),
   ((infix_plpl l (Nil :(list a))) = l).
 
 (* Why3 assumption *)
-Fixpoint length {a:Type} {a_WT:WhyType a} (l:(list a)) {struct l}: Z :=
+Fixpoint length {a:Type} {a_WT:WhyType a}(l:(list a)) {struct l}: Z :=
   match l with
   | Nil => 0%Z
   | (Cons _ r) => (1%Z + (length r))%Z
@@ -106,7 +126,7 @@ Axiom Append_length : forall {a:Type} {a_WT:WhyType a}, forall (l1:(list a))
   l2)) = ((length l1) + (length l2))%Z).
 
 (* Why3 assumption *)
-Fixpoint mem {a:Type} {a_WT:WhyType a} (x:a) (l:(list a)) {struct l}: Prop :=
+Fixpoint mem {a:Type} {a_WT:WhyType a}(x:a) (l:(list a)) {struct l}: Prop :=
   match l with
   | Nil => False
   | (Cons y r) => (x = y) \/ (mem x r)
@@ -121,7 +141,7 @@ Axiom mem_decomp : forall {a:Type} {a_WT:WhyType a}, forall (x:a) (l:(list
   (l = (infix_plpl l1 (Cons x l2))).
 
 (* Why3 assumption *)
-Fixpoint inorder {a:Type} {a_WT:WhyType a} (t:(tree a)) {struct t}: (list
+Fixpoint inorder {a:Type} {a_WT:WhyType a}(t:(tree a)) {struct t}: (list
   a) :=
   match t with
   | Empty => (Nil :(list a))
@@ -132,26 +152,22 @@ Fixpoint inorder {a:Type} {a_WT:WhyType a} (t:(tree a)) {struct t}: (list
 Inductive distinct{a:Type} {a_WT:WhyType a}  : (list a) -> Prop :=
   | distinct_zero : (distinct (Nil :(list a)))
   | distinct_one : forall (x:a), (distinct (Cons x (Nil :(list a))))
-  | distinct_many : forall (x:a) (l:(list a)), (~ (mem x l)) -> ((distinct
-      l) -> (distinct (Cons x l))).
+  | distinct_many : forall (x:a) (l:(list a)), (~ (mem x l)) ->
+      ((distinct l) -> (distinct (Cons x l))).
 
 Axiom distinct_append : forall {a:Type} {a_WT:WhyType a}, forall (l1:(list
-  a)) (l2:(list a)), (distinct l1) -> ((distinct l2) -> ((forall (x:a), (mem
-  x l1) -> ~ (mem x l2)) -> (distinct (infix_plpl l1 l2)))).
+  a)) (l2:(list a)), (distinct l1) -> ((distinct l2) -> ((forall (x:a),
+  (mem x l1) -> ~ (mem x l2)) -> (distinct (infix_plpl l1 l2)))).
 
 (* Why3 assumption *)
-Inductive tree1 : (map.Map.map pointer node) -> pointer -> (tree
-  pointer) -> Prop :=
-  | leaf : forall (m:(map.Map.map pointer node)), (tree1 m null (Empty :(tree
-      pointer)))
-  | node1 : forall (m:(map.Map.map pointer node)) (p:pointer) (l:(tree
-      pointer)) (r:(tree pointer)), (~ (p = null)) -> ((tree1 m
-      (left1 (map.Map.get m p)) l) -> ((tree1 m (right1 (map.Map.get m p))
-      r) -> (tree1 m p (Node l p r)))).
+Inductive istree : (map loc node) -> loc -> (tree loc) -> Prop :=
+  | leaf : forall (m:(map loc node)), (istree m null (Empty :(tree loc)))
+  | node1 : forall (m:(map loc node)) (p:loc) (l:(tree loc)) (r:(tree loc)),
+      (~ (p = null)) -> ((istree m (left1 (get m p)) l) -> ((istree m
+      (right1 (get m p)) r) -> (istree m p (Node l p r)))).
 
 (* Why3 assumption *)
-Inductive zipper
-  (a:Type) {a_WT:WhyType a} :=
+Inductive zipper (a:Type) {a_WT:WhyType a} :=
   | Top : zipper a
   | Left : (zipper a) -> a -> (tree a) -> zipper a.
 Axiom zipper_WhyType : forall (a:Type) {a_WT:WhyType a}, WhyType (zipper a).
@@ -160,7 +176,7 @@ Implicit Arguments Top [[a] [a_WT]].
 Implicit Arguments Left [[a] [a_WT]].
 
 (* Why3 assumption *)
-Fixpoint zip {a:Type} {a_WT:WhyType a} (t:(tree a)) (z:(zipper
+Fixpoint zip {a:Type} {a_WT:WhyType a}(t:(tree a)) (z:(zipper
   a)) {struct z}: (tree a) :=
   match z with
   | Top => t
@@ -177,7 +193,7 @@ Require Import Why3.
 Ltac ae := why3 "Alt-Ergo,0.95," timelimit 3.
 
 Lemma distinct1:
-  forall (p pp: pointer) (pr ppr: tree pointer),
+  forall (p pp: loc) (pr ppr: tree loc),
     distinct (Cons p (infix_plpl (inorder pr) (Cons pp (inorder ppr)))) ->
     p <> pp.
   Proof.
@@ -187,7 +203,7 @@ Lemma distinct1:
 Lemma distinct2:
   forall m p p' n t, 
     let m' := Map.set m p' n in
-    tree1 m p t -> ~ (mem p' (inorder t)) -> tree1 m' p t.
+    istree m p t -> ~ (mem p' (inorder t)) -> istree m' p t.
   Proof.
     induction 1; simpl.
     ae.
@@ -202,27 +218,27 @@ Lemma distinct2:
   Qed.
 
 Lemma distinct3:
-  forall (pp: pointer) (l1 l2: list pointer),
+  forall (pp: loc) (l1 l2: list loc),
   distinct (infix_plpl l1 (Cons pp l2)) -> ~ (mem pp l1).
 Proof.
 induction l1; simpl; ae.
 Qed.
 
 Lemma distinct4:
-  forall (pp: pointer) (l1 l2: list pointer),
+  forall (pp: loc) (l1 l2: list loc),
   distinct (infix_plpl l1 (Cons pp l2)) -> ~ (mem pp l2).
 Proof.
 induction l1; simpl; ae.
 Qed.
 
 Lemma distinct_append1:
-  forall (l1 l2: list pointer), distinct (infix_plpl l1 l2) -> distinct l1.
+  forall (l1 l2: list loc), distinct (infix_plpl l1 l2) -> distinct l1.
 Proof.
   induction l1; simpl; ae.
 Qed.
 
 Lemma distinct5:
-  forall z (p: pointer) (l r: tree pointer),
+  forall z (p: loc) (l r: tree loc),
   distinct (inorder (zip (Node l p r) z)) -> distinct (inorder (Node l p r)).
 Proof.
 induction z.
@@ -233,9 +249,9 @@ generalize (IHz a (Node l p r) t); clear IHz.
 ae.
 Qed.
 
-Lemma tree1_zip:
+Lemma istree_zip:
   forall m t z l r pp,
-  tree1 m t (zip (Node l pp r) z) -> tree1 m pp (Node l pp r).
+  istree m t (zip (Node l pp r) z) -> istree m pp (Node l pp r).
 Proof.
 induction z; simpl.
 ae.
@@ -245,13 +261,13 @@ generalize (IHz (Node l pp r) t0 a).
 ae.
 Qed.
 
-Lemma tree1_zip_2:
+Lemma istree_zip_2:
   forall m n a z t pp l r tr',
-  tree1 m t (zip (Node l pp r) z) ->
+  istree m t (zip (Node l pp r) z) ->
   distinct (inorder (zip (Node l pp r) z)) ->
   mem a (inorder (Node l pp r)) -> let m' := Map.set m a n in
-  tree1 m' pp tr' ->
-  tree1 m' t (zip tr' z).
+  istree m' pp tr' ->
+  istree m' t (zip tr' z).
 Proof.
 induction z; simpl.
 ae.
@@ -265,20 +281,20 @@ apply node1.
 why3 "cvc3".
 assert (left1 (Map.get (Map.set m a n) a0) = pp).
 rewrite Map.Select_neq.
-  generalize (tree1_zip _ _ _ _ _ _ H).
+  generalize (istree_zip _ _ _ _ _ _ H).
   inversion 1.
   inversion H11; auto.
 assumption.
 ae.
 assert (right1 (Map.get (Map.set m a n) a0) = right1 (Map.get m a0)).
 rewrite Map.Select_neq.
-  generalize (tree1_zip _ _ _ _ _ _ H).
+  generalize (istree_zip _ _ _ _ _ _ H).
   inversion 1.
   inversion H11; auto.
 assumption.
 rewrite H5; clear H5.
 apply distinct2.
-generalize (tree1_zip _ _ _ _ _ _ H).
+generalize (istree_zip _ _ _ _ _ _ H).
 inversion 1.
 ae.
 clear H4 H2 H H3.
@@ -297,20 +313,19 @@ ae.
 Qed.
 
 (* Why3 goal *)
-Theorem main_lemma : forall (m:(map.Map.map pointer node)) (t:pointer)
-  (pp:pointer) (p:pointer) (ppr:(tree pointer)) (pr:(tree pointer))
-  (z:(zipper pointer)), let it := (zip (Node (Node (Empty :(tree pointer)) p
-  pr) pp ppr) z) in ((tree1 m t it) -> ((distinct (inorder it)) -> (tree1
-  (map.Map.set m pp (mk_node (right1 (map.Map.get m p))
-  (right1 (map.Map.get m pp)) (data (map.Map.get m pp)))) t (zip (Node pr pp
-  ppr) z)))).
+Theorem main_lemma : forall (m:(map loc node)) (t:loc) (pp:loc) (p:loc)
+  (ppr:(tree loc)) (pr:(tree loc)) (z:(zipper loc)), let it :=
+  (zip (Node (Node (Empty :(tree loc)) p pr) pp ppr) z) in ((istree m t
+  it) -> ((distinct (inorder it)) -> (istree (set m pp
+  (mk_node (right1 (get m p)) (right1 (get m pp)) (data (get m pp)))) t
+  (zip (Node pr pp ppr) z)))).
 intros m t pp p ppr pr z it h1 h2.
 pose (m' := (Map.set m pp
      (mk_node (right1 (Map.get m p)) (right1 (Map.get m pp))
         (data (Map.get m pp))))).
-assert (tree1 m' pp (Node pr pp ppr)).
-assert (tree1 m pp (Node (Node (Empty:tree pointer) p pr) pp ppr)) by ae.
-assert (tree1 m' pp (Node pr pp ppr)).
+assert (istree m' pp (Node pr pp ppr)).
+assert (istree m pp (Node (Node (Empty:tree loc) p pr) pp ppr)) by ae.
+assert (istree m' pp (Node pr pp ppr)).
 inversion H; simpl.
 apply node1.
 assumption.
@@ -329,8 +344,8 @@ apply distinct2.
 ae.
 why3 "cvc3" timelimit 3.
 assumption.
-Print tree1_zip_2.
-apply tree1_zip_2 with (l := (Node (Empty:tree pointer) p pr)) (r := ppr)
+Print istree_zip_2.
+apply istree_zip_2 with (l := (Node (Empty:tree loc) p pr)) (r := ppr)
   (pp := pp); try
 assumption.
 ae.
